Everything seems fine before Subst

Capless/Subcapturing.lean
@@ -12,13 +12,14 @@ namespace Capless
 
 
 inductive CaptureKind : Context n m k -> CaptureSet n k -> Kind -> Prop where
-  | var : Context.Bound Γ x (S^C) -> CaptureKind Γ C K -> CaptureKind Γ {x=x | L} (L.intersect K)
+  | var : Context.Bound Γ x (S^C) -> CaptureKind Γ (C.proj L) K -> CaptureKind Γ {x=x | L} K
   | label : Context.LBound Γ x c S -> CaptureKind Γ {x=x|K} (K.intersect (.node c []))
   | cvar : Context.CBound Γ c (.bound (.kind K)) -> CaptureKind Γ {c=c|L} (L.intersect K)
-  | cbound : Context.CBound Γ c (.bound (.upper C)) -> CaptureKind Γ C K -> CaptureKind Γ {c=c | L} (L.intersect K)
-  | cinstr : Context.CBound Γ c (.inst C) -> CaptureKind Γ C K -> CaptureKind Γ {c=c | L} (L.intersect K)
+  | cbound : Context.CBound Γ c (.bound (.upper C)) -> CaptureKind Γ (C.proj L) K -> CaptureKind Γ {c=c | L} K
+  | cinstr : Context.CBound Γ c (.inst C) -> CaptureKind Γ (C.proj L) K -> CaptureKind Γ {c=c | L} K
   | sub : Kind.Subkind K L -> CaptureKind Γ C K -> CaptureKind Γ C L
   | empty : CaptureKind Γ .empty K
+  | absurd : L.IsEmpty -> CaptureKind Γ (.singleton s L) K
   | union : CaptureKind Γ C1 K -> CaptureKind Γ C2 K -> CaptureKind Γ (C1 ∪ C2) K
 
 inductive Subcapt : Context n m k -> CaptureSet n k -> CaptureSet n k -> Prop where
@@ -48,7 +49,11 @@ inductive Subcapt : Context n m k -> CaptureSet n k -> CaptureSet n k -> Prop wh
 | subkind : K.Subkind L -> Subcapt Γ (.singleton s K) (.singleton s L)
 | proj_absurd : L.IsEmpty -> Subcapt Γ (.singleton s L) .empty
 | proj_split : Subcapt Γ (.singleton s (.union K1 K2)) (.union (.singleton s K1) (.singleton s K2))
-| proj_merge : Subcapt Γ (.union (.singleton s K1) (.singleton s K2)) (.singleton s (.union K1 K2))
+
+theorem Subcapt.proj_merge : Subcapt Γ (.union (.singleton s K1) (.singleton s K2)) (.singleton s (.union K1 K2)) := by
+  apply union
+  . apply subkind $ .union_rl (K2:=K2)
+  . apply subkind .union_rr
 
 notation:50 Γ " ⊢ " C1 " <:c " C2 => Subcapt Γ C1 C2
 notation:50 Γ " ⊢ " C " :k " K => CaptureKind Γ C K
