Capless/Subcapturing/Basic.lean
@@ -76,11 +76,6 @@ theorem Subcapt.union_l_inv' (hs : Subcapt Γ C D) (heq : C = (C1 ∪ C2)) : Sub
     apply And.intro <;> apply! trans _ (.cinstl hb)
   case union =>
     injections; subst_vars; apply And.intro <;> assumption
-  case proj_merge =>
-    have ⟨_, _⟩ := heq; subst_vars; simp_all
-    apply And.intro <;> apply subkind
-    apply Kind.Subkind.union_rl
-    apply Kind.Subkind.union_rr
 
 theorem Subcapt.union_l_inv (hs : Subcapt Γ (C1 ∪ C2) D) : Subcapt Γ C1 D ∧ Subcapt Γ C2 D := hs.union_l_inv' $ .refl (a := C1 ∪ C2)
 theorem CaptureKind.union_l_inv (hk : CaptureKind Γ (C1 ∪ C2) K) : CaptureKind Γ C1 K ∧ CaptureKind Γ C2 K := hk.union_l_inv' $ .refl (a := C1 ∪ C2)
@@ -97,6 +92,318 @@ theorem Subcapt.proj_absurd_set {C : CaptureSet n k} (he : L.IsEmpty) : Subcapt 
     apply trans
     apply subkind Kind.Intersect.subkind_r
     apply! proj_absurd
+
+theorem CaptureKind.subset
+  (hk : CaptureKind Γ C2 K)
+  (hs : C1 ⊆ C2)
+  : CaptureKind Γ C1 K := by
+  induction hs
+  case empty => apply empty
+  case rfl => assumption
+  case union_l ha hb => apply! union (ha _) (hb _)
+  case union_rl ih =>
+    have ⟨_, _⟩ := hk.union_l_inv
+    apply! ih
+  case union_rr ih =>
+    have ⟨_, _⟩ := hk.union_l_inv
+    apply! ih
+
+theorem CaptureKind.subkind_proj
+  (hk : CaptureKind Γ (.proj C K2) K)
+  (hs : Kind.Subkind K1 K2)
+  : CaptureKind Γ (.proj C K1) K := by
+  generalize h : C.proj K2 = D at hk
+  induction hk generalizing C K2 K1
+  case var hb hk ih =>
+    unfold CaptureSet.proj at h; split at h <;> simp at h
+    have ⟨_, _⟩ := h; subst_vars; simp_all
+    apply var hb
+    apply ih _ (.refl _)
+    apply Kind.Intersect.with_subkind hs
+  case label hb =>
+    unfold CaptureSet.proj at h; split at h <;> simp at h
+    have ⟨_, _⟩ := h; subst_vars; simp_all
+    apply sub
+    apply (Kind.Intersect.with_subkind_r (Kind.Intersect.with_subkind hs))
+    apply! label
+  case cvar hb =>
+    unfold CaptureSet.proj at h; split at h <;> simp at h
+    have ⟨_, _⟩ := h; subst_vars; simp_all
+    apply sub
+    apply (Kind.Intersect.with_subkind_r (Kind.Intersect.with_subkind hs))
+    apply! cvar
+  case cbound hb hk ih =>
+    unfold CaptureSet.proj at h; split at h <;> simp at h
+    have ⟨_, _⟩ := h; subst_vars; simp_all
+    apply cbound hb
+    apply ih _ (.refl _)
+    apply Kind.Intersect.with_subkind hs
+  case cinstr hb hk ih =>
+    unfold CaptureSet.proj at h; split at h <;> simp at h
+    have ⟨_, _⟩ := h; subst_vars; simp_all
+    apply cinstr hb
+    apply ih _ (.refl _)
+    apply Kind.Intersect.with_subkind hs
+  case sub hs2 hk ih =>
+    subst_vars
+    apply sub hs2
+    apply ih hs (.refl _)
+  case empty =>
+    unfold CaptureSet.proj at h; split at h <;> simp at h
+    apply empty
+  case absurd he =>
+    unfold CaptureSet.proj at h; split at h <;> simp at h
+    have ⟨_, _⟩ := h; subst_vars; simp_all
+    apply absurd
+    apply Kind.Subkind.of_empty (Kind.Intersect.with_subkind hs) he
+  case union ha hb =>
+    unfold CaptureSet.proj at h; split at h <;> simp at h
+    have ⟨_, _⟩ := h; subst_vars; simp_all
+    apply union (ha hs (.refl _)) (hb hs (.refl _))
+
+
+
+
+
+
+
+theorem CaptureKind.subkind_singleton
+  (hs : CaptureKind Γ (.singleton s K2) K)
+  (hsub : K1.Subkind K2)
+  : CaptureKind Γ (.singleton s K1) K := by
+  rw [← Kind.Intersect.top_l (K:=K2)] at hs
+  rw [← Kind.Intersect.top_l (K:=K1)]
+  rw [← CaptureSet.proj] at hs
+  rw [← CaptureSet.proj]
+  apply! subkind_proj
+
+theorem CaptureKind.absurd_set {C : CaptureSet n k}
+  (he : L.IsEmpty)
+  : CaptureKind Γ (C.proj L) K := by
+  induction C
+  case empty => apply empty
+  case union ha hb => apply! union
+  case singleton => simp; apply absurd; apply Kind.Intersect.is_empty_r he
+
+theorem CaptureKind.var_lookup_inv
+  (hk : CaptureKind Γ {x=x|L} K)
+  (hb : Γ.Bound x S^C)
+  : L.IsEmpty ∨ CaptureKind Γ (C.proj L) K := by
+  generalize h : {x=x|L} = D at hk
+  induction hk <;> cases h
+  case var K hb2 hk ih =>
+    cases Context.bound_injective hb hb2
+    right; assumption
+  case label hb2 => cases Context.bound_lbound_absurd hb hb2
+  case sub hs hk ih =>
+    cases ih hb (.refl _)
+    case inl => left; assumption
+    case inr h => right; apply! sub
+  case absurd => aesop
+
+theorem CaptureKind.label_lookup_inv
+  (hs : CaptureKind Γ {x=x|K1} K)
+  (hb : Γ.LBound x c S)
+  : K1.IsEmpty ∨ (K1.intersect (.classifier c)).Subkind K := by
+  generalize h : {x=x|K1} = D at hs
+  induction hs <;> cases h
+  case var hb1 hk ih => cases Context.bound_lbound_absurd hb1 hb
+  case label hb1 =>
+    cases Context.lbound_inj hb hb1; subst_vars
+    right; exact .rfl
+  case sub hs1 _ ih =>
+    cases ih hb (.refl _)
+    case inl => aesop
+    case inr h => right; exact .trans h hs1
+  case absurd => aesop
+
+theorem CaptureKind.cbound_lookup_inv
+  (hs : CaptureKind Γ {c=c|L} K)
+  (hb : Γ.CBound c (.bound (.upper C)))
+  : L.IsEmpty ∨ CaptureKind Γ (C.proj L) K := by
+  generalize h : {c=c|L} = D at hs
+  induction hs <;> cases h
+  case cvar hb2 => cases Context.cbound_injective hb hb2
+  case cbound hb2 hk ih =>
+    cases Context.cbound_injective hb hb2
+    right; assumption
+  case cinstr hb2 hk ih => cases Context.cbound_injective hb hb2
+  case sub hs hk ih =>
+    cases ih hb (.refl _)
+    case inl => left; assumption
+    case inr h => right; apply! sub
+  case absurd => aesop
+
+theorem CaptureKind.ckind_lookup_inv
+  (hs : CaptureKind Γ {c=c|L} K)
+  (hb : Γ.CBound c (.bound (.kind K1)))
+  : L.IsEmpty ∨ (L.intersect K1).Subkind K := by
+  generalize h : {c=c|L} = D at hs
+  induction hs <;> cases h
+  case cvar hb2 =>
+    cases Context.cbound_injective hb hb2
+    right; exact .rfl
+  case cbound hb2 hk ih => cases Context.cbound_injective hb hb2
+  case cinstr hb2 hk ih => cases Context.cbound_injective hb hb2
+  case sub hs1 _ ih =>
+    cases ih hb (.refl _)
+    case inl => aesop
+    case inr h => right; exact .trans h hs1
+  case absurd => aesop
+
+theorem CaptureKind.cinst_lookup_inv
+  (hs : CaptureKind Γ {c=c|L} K)
+  (hb : Γ.CBound c (.inst C))
+  : L.IsEmpty ∨ CaptureKind Γ (C.proj L) K := by
+  generalize h : {c=c|L} = D at hs
+  induction hs <;> cases h
+  case cvar hb2 => cases Context.cbound_injective hb hb2
+  case cbound hb2 hk ih => cases Context.cbound_injective hb hb2
+  case cinstr hb2 hk ih =>
+    cases Context.cbound_injective hb hb2
+    right; assumption
+  case sub hs hk ih =>
+    cases ih hb (.refl _)
+    case inl => left; assumption
+    case inr h => right; apply! sub
+  case absurd => aesop
+
+theorem CaptureKind.proj_merge
+  (hk1 : CaptureKind Γ (.proj C K1) L1)
+  (hk2 : CaptureKind Γ (.proj C K2) L2)
+  (hs1 : L1.Subkind L)
+  (hs2 : L2.Subkind L)
+  : CaptureKind Γ (.proj C (K1.union K2)) L := by
+  generalize h : C.proj K1 = D at hk1
+  induction hk1 generalizing C K1 K2
+  case var x _ _ _ K hb hk1 ih =>
+    unfold CaptureSet.proj at h; split at h <;> simp at h
+    have ⟨_, _⟩ := h; subst_vars; simp_all
+    apply var hb
+    apply subkind_proj _ Kind.Intersect.union_r_subkind
+    cases hk2.var_lookup_inv hb
+    case inl h =>
+      apply sub hs1
+      apply subkind_proj hk1
+      apply! Kind.Subkind.union_l .rfl $ .is_empty_l _
+    case inr h => apply ih h (.refl _)
+  case label hb =>
+    unfold CaptureSet.proj at h; split at h <;> simp at h
+    have ⟨_, _⟩ := h; subst_vars; simp_all
+    cases hk2.label_lookup_inv hb
+    case inl h =>
+      apply sub hs1
+      apply subkind_singleton (label hb)
+      apply Kind.Intersect.union_r_subkind.trans
+      apply Kind.Subkind.union_l .rfl $ .is_empty_l h
+    case inr h =>
+      apply sub
+      exact .union_l hs1 (.trans h hs2)
+      apply sub Kind.Intersect.union_l_subkind
+      apply sub $ Kind.Intersect.with_subkind_r Kind.Intersect.union_r_subkind
+      apply label hb
+  case cvar hb =>
+    unfold CaptureSet.proj at h; split at h <;> simp at h
+    have ⟨_, _⟩ := h; subst_vars; simp_all
+    cases hk2.ckind_lookup_inv hb
+    case inl h =>
+      -- h : (p.intersect K2).IsEmpty
+      apply sub hs1
+      apply sub $ Kind.Intersect.with_subkind_r $
+        Kind.Subkind.trans Kind.Intersect.union_r_subkind $
+        Kind.Subkind.union_l .rfl $ Kind.Subkind.is_empty_l h
+      apply cvar hb
+    case inr h =>
+      -- h : ((p.intersect K2).intersect K).Subkind L2
+      apply sub
+      exact .union_l hs1 (.trans h hs2)
+      apply sub Kind.Intersect.union_l_subkind
+      apply sub $ Kind.Intersect.with_subkind_r Kind.Intersect.union_r_subkind
+      apply cvar hb
+  case cbound hb hk1 ih =>
+    unfold CaptureSet.proj at h; split at h <;> simp at h
+    have ⟨_, _⟩ := h; subst_vars; simp_all
+    apply cbound hb
+    apply subkind_proj _ Kind.Intersect.union_r_subkind
+    cases hk2.cbound_lookup_inv hb
+    case inl h =>
+      apply sub hs1
+      apply subkind_proj hk1
+      apply Kind.Subkind.union_l .rfl $ Kind.Subkind.is_empty_l h
+    case inr h => apply ih h (.refl _)
+  case cinstr hb hk1 ih =>
+    unfold CaptureSet.proj at h; split at h <;> simp at h
+    have ⟨_, _⟩ := h; subst_vars; simp_all
+    apply cinstr hb
+    apply subkind_proj _ Kind.Intersect.union_r_subkind
+    cases hk2.cinst_lookup_inv hb
+    case inl h =>
+      apply sub hs1
+      apply subkind_proj hk1
+      apply Kind.Subkind.union_l .rfl $ Kind.Subkind.is_empty_l h
+    case inr h => apply ih h (.refl _)
+  case sub hs hk1 ih =>
+    subst_vars
+    apply ih hk2
+    exact .trans hs hs1
+    rfl
+  case empty =>
+    unfold CaptureSet.proj at h; split at h <;> simp at h
+    apply empty
+  case absurd =>
+    unfold CaptureSet.proj at h; split at h <;> simp at h
+    have ⟨_, _⟩ := h; subst_vars; simp_all
+    apply subkind_singleton
+    apply sub hs2 hk2
+    apply Kind.Subkind.trans
+    . apply Kind.Intersect.union_r_subkind
+    . apply Kind.Subkind.union_l _ .rfl
+      . apply! Kind.Subkind.is_empty_l
+  case union ha hb =>
+    unfold CaptureSet.proj at h; split at h <;> simp at h
+    have ⟨_, _⟩ := h; subst_vars; simp_all
+    have ⟨_, _⟩ := hk2.union_l_inv
+    apply! union (ha _ $ .refl _) (hb _ $ .refl _)
+
+theorem CaptureKind.proj_merge_singleton
+  (hs1 : CaptureKind Γ (.singleton s K1) K)
+  (hs2 : CaptureKind Γ (.singleton s K2) K)
+  : CaptureKind Γ (.singleton s (K1.union K2)) K := by
+  rw [← Kind.Intersect.top_l (K:=K1)] at hs1
+  rw [← Kind.Intersect.top_l (K:=K2)] at hs2
+  rw [← CaptureSet.proj] at hs1 hs2
+  rw [← Kind.Intersect.top_l (K:=K1.union K2), ← CaptureSet.proj]
+  exact proj_merge hs1 hs2 .rfl .rfl
+
+theorem CaptureKind.subcapt
+  (hk : CaptureKind Γ C2 K)
+  (hs : Subcapt Γ C1 C2)
+  : CaptureKind Γ C1 K := by
+  induction hs generalizing K
+  case trans ha hb => apply ha; apply! hb
+  case subset => apply! hk.subset
+  case union ha hb => apply! union (ha _) (hb _)
+  case var hb => apply! var
+  case cinstl c C L hb =>
+    generalize h : {c=c|L} = D at hk
+    induction hk <;> try cases h
+    case cvar hb1 => cases Context.cbound_injective hb hb1
+    case cbound hb1 hk ih => cases Context.cbound_injective hb hb1
+    case cinstr hb1 hk ih => cases Context.cbound_injective hb hb1; assumption
+    case sub hs hk ih => apply sub hs; apply ih hb; rfl
+    case absurd he => apply! absurd_set
+  case cinstr => apply! cinstr
+  case cbound => apply! cbound
+  case subkind K1 L hs =>
+    rw [← Kind.Intersect.top_l (K:=L)] at hk
+    rw [← Kind.Intersect.top_l (K:=K1)]
+    rw [← CaptureSet.proj] at hk
+    rw [← CaptureSet.proj]
+    apply subkind_proj hk hs
+  case proj_absurd he => apply! absurd
+  case proj_split =>
+    have ⟨_, _⟩ := hk.union_l_inv
+    apply! proj_merge_singleton
 
 -- theorem CaptureKind.proj_kind : CaptureKind Γ (.proj C K) K := by
 --   induction C
