Capless/Subtyping/Basic.lean
@@ -15,9 +15,9 @@ theorem Subbound.refl {B : CBound n k} :
   Subbound Γ B B := by
   cases B <;> constructor
   case upper =>
-    apply Subcapt.refl
+    apply Subcapt.rfl
   case kind =>
-    apply Kind.subkind_refl
+    apply Kind.Subkind.rfl
 
 theorem Subbound.trans
   (h1 : Subbound Γ B1 B2)
@@ -26,7 +26,7 @@ theorem Subbound.trans
   cases h1 <;> cases h2 <;> constructor
   apply Subcapt.trans <;> easy
   rename_i hsub K hk
-  apply CaptureKind.csub hsub hk
+  apply hk.subcapt hsub
   rename_i k1 k2 h1 k3 h2
   apply Kind.Subkind.trans h1 h2
   rename_i hk K2 hs
@@ -64,7 +64,7 @@ theorem ESubtyp.ex_inv_subcapt
 theorem CSubtyp.refl :
   CSubtyp Γ T T := by
   cases T; apply capt
-  { apply Subcapt.refl }
+  { apply Subcapt.rfl }
   { apply SSubtyp.refl }
 
 theorem ESubtyp.refl :
