Capless/Weakening/Typing.lean
@@ -38,7 +38,7 @@ theorem Typed.weaken
 
 theorem Typed.lweaken
   (h : Typed Γ t E Ct) :
-  Typed (Γ.label S) t.weaken E.weaken Ct.weaken := by
+  Typed (Γ.label c S) t.weaken E.weaken Ct.weaken := by
   simp [Term.weaken, EType.weaken]
   apply h.rename
   apply VarMap.lweaken
@@ -51,7 +51,7 @@ theorem Typed.weaken_ext {Γ : Context n m k}
 
 theorem Typed.lweaken_ext {Γ : Context n m k}
   (h : Typed (Γ.var T) t E Ct) :
-  Typed ((Γ.label P).var T.weaken) t.weaken1 E.weaken1 Ct.weaken1 := by
+  Typed ((Γ.label c P).var T.weaken) t.weaken1 E.weaken1 Ct.weaken1 := by
   simp [Term.weaken1, EType.weaken1]
   apply h.rename VarMap.lweaken_ext
 
@@ -63,7 +63,7 @@ theorem Typed.weaken_cext_ext {Γ : Context n m k}
 
 theorem Typed.lweaken_cext_ext {Γ : Context n m k}
   (h : Typed ((Γ.cvar (CBinding.bound B)).var T) t E Ct) :
-  Typed (((Γ.label P).cvar (CBinding.bound B.weaken)).var T.weaken) t.weaken1 E.weaken1 Ct.weaken1 := by
+  Typed (((Γ.label c P).cvar (CBinding.bound B.weaken)).var T.weaken) t.weaken1 E.weaken1 Ct.weaken1 := by
   simp [Term.weaken1, EType.weaken1]
   apply h.rename VarMap.lweaken_cext_ext
 
